src/goose_lang/crash_borrow.v
@@ -1,0 +1,121 @@
+From Perennial.program_logic Require Import staged_invariant.
+From Perennial.goose_lang Require Import crash_modality lifting wpr_lifting.
+
+
+Section crash_borrow_def.
+Context `{ext:ffi_syntax}.
+Context `{ffi_sem: ffi_semantics}.
+Context `{!ffi_interp ffi}.
+
+Context `{!heapGS Σ}.
+Context `{!stagedG Σ}.
+
+Global Instance later_tokG_heap : later_tokG (heapG_irisG).
+Proof.
+  refine {| later_tok := cred_frag 1 |}.
+  - iIntros (g ns mj D κ) "(Hg&Hfrag)".
+    iDestruct "Hg" as "(Hffi&Hinv&Hcred&Htok)".
+    iMod (cred_interp_decr with "[$]") as (ns' ->) "(Hauth&Hfrag)".
+    iExists ns'. iModIntro; iSplit; first done.
+    iFrame. iDestruct "Hauth" as "($&_)".
+  - iIntros (g ns mj D κ) "Hg".
+    iDestruct "Hg" as "(Hffi&Hinv&(Hcred&H0)&Htok)".
+    iMod (cred_interp_incr with "[$]") as "(Hauth&Hfrag)".
+    iFrame. eauto.
+  - intros n1 n2 Hlt => /=.
+    transitivity (3 ^ (1 + (n1 + 1)))%nat; last first.
+    { apply Nat.pow_le_mono_r; lia. }
+    rewrite [a in _ _ a]Nat.pow_add_r.
+    rewrite [a in _ _ a]/=.
+    transitivity (2 + 3^(n1 + 1) + 3^(n1 + 1))%nat; first by lia.
+    rewrite plus_0_r -plus_assoc.
+    apply plus_le_compat_r.
+    clear.
+    transitivity (2 ^ 1)%nat; first by auto.
+    etransitivity; last eapply (Nat.pow_le_mono_r _ 1); try (simpl; lia).
+  - intros n1 n2 Hlt => /=. lia.
+Qed.
+
+Lemma ownfCP_inf_le1 γ (q : Qp) (E : coPset) :
+  ownfCP_inf γ q E -∗ ⌜ q ≤ 1 ⌝%Qp.
+Proof.
+  iDestruct 1 as "(%Hinf&Hown)".
+  iDestruct (own_valid with "Hown") as %Hval.
+  iPureIntro.
+  destruct Hval as (Hval&Hdom).
+  specialize (Hval (coPpick E)).
+  rewrite /= decide_True in Hval => //=.
+  apply coPpick_elem_of.
+  intros ?. apply set_not_infinite_finite in Hinf; eauto.
+Qed.
+
+Lemma ownfCP_disj1 γ q1 D E :
+  ownfCP γ q1 D ∗ ownfCP_inf γ 1 E -∗ ⌜ E ## D ⌝.
+Proof.
+  iIntros. iDestruct (ownfCP_disj with "[$]") as %Hcases. iPureIntro.
+  destruct Hcases as [Hdisj|Hbad]; auto. exfalso.
+  move: Hbad. rewrite frac_valid Qp_le_ngt => Hnlt. apply Hnlt.
+  apply Qp_lt_add_r.
+Qed.
+
+Lemma ownfCP_disj_gt2 γ q D E :
+  (/2 < q)%Qp →
+  ownfCP γ q D ∗ ownfCP_inf γ q E -∗ ⌜ E ## D ⌝.
+Proof.
+  iIntros. iDestruct (ownfCP_disj with "[$]") as %Hcases. iPureIntro.
+  destruct Hcases as [Hdisj|Hbad]; auto. exfalso.
+  move: Hbad. rewrite frac_valid Qp_le_ngt => Hnlt. apply Hnlt.
+  rewrite -Qp_inv_half_half.
+  apply Qp_add_lt_mono; auto.
+Qed.
+
+Global Instance pri_invG_heap : pri_invG (heapG_irisG).
+Proof.
+  refine {| pri_inv_tok := λ q E, pinv_tok_inf q E |}; rewrite /pinv_tok_inf.
+  - iIntros (??) "($&?)".
+  - iIntros (???) "H". by rewrite ownfCP_inf_op_plus.
+  - iIntros (???). rewrite ownfCP_inf_op_plus. by iIntros "$ $".
+  - iIntros (q E) "H". by iApply (ownfCP_inf_le1).
+  - iIntros (?????) "Hg". iDestruct "Hg" as "(?&?&?&?&?)". eauto.
+  - iIntros (??????) "%Hlt Hg". iDestruct "Hg" as "(?&?&?&%Hle2&Hp)".
+    iDestruct (ownfCP_op_plus with "Hp") as "(Hp1&$)".
+    iFrame. iSplit.
+    { iPureIntro. split; auto. transitivity (q1 + q2)%Qp; last by naive_solver.
+      apply Qp_le_add_r. }
+    iIntros (???) "Hg". iDestruct "Hg" as "(?&?&?&%Hle2'&Hp)".
+    iFrame. iSplit; first auto.
+    iApply ownfCP_op_plus. iFrame.
+  - iIntros (?????) "%Hlt (Hg&Hp')". iDestruct "Hg" as "(?&?&?&%Hle2&Hp)".
+    iFrame. iDestruct "Hp'" as "(%Hinf&Hp')".
+    iDestruct (ownfCP_op_plus with "[$Hp' $Hp]") as "Hp".
+    iDestruct (ownfCP_inf_le1 with "[$Hp //]") as %Hle3.
+    iFrame. iPureIntro.
+    split; auto. transitivity q2; first naive_solver.
+    apply Qp_lt_add_r.
+  - iIntros (g ns q D κ) "Hg".
+    iMod (ownfCP_inf_init (coPset_name credit_cr_names)) as (E) "H".
+    iDestruct "Hg" as "($&$&$&$&Hp)".
+    iDestruct "H" as "(%Hinf&H)".
+    iExists E.
+    iDestruct (ownfCP_disj1 with "[$Hp H]") as %Hdisj.
+    { iFrame; eauto. }
+    iFrame. eauto.
+  - iIntros (E g ns q D κ) "(Hp&Hg)".
+    iDestruct "Hg" as "($&$&$&%Hle&Hp')".
+    iFrame "%".
+    iDestruct (ownfCP_disj_gt2 with "[$Hp $Hp']") as %Hdisj; first naive_solver.
+    iDestruct "Hp" as "(Hinf&Hp)".
+    iModIntro. iApply ownfCP_op_union; auto.
+    iFrame.
+  - iIntros (E g ns q D κ) "((%Hdisj&%Hinf)&Hg)".
+    iDestruct "Hg" as "($&$&$&$&Hp)".
+    iDestruct (ownfCP_op_union with "Hp") as "($&$)"; auto.
+  - iIntros (g ns q1 q2 D κ E) "(Hg&Hp')".
+    iDestruct "Hg" as "(?&?&?&%Hle&Hp)".
+    iApply (ownfCP_disj with "[$]").
+Qed.
+
+Definition crash_borrow Ps Pc : iProp Σ :=
+  (staged_value_idle ⊤ Ps True%I Pc ∗ later_tok ∗ later_tok ∗ later_tok).
+
+End crash_borrow_def.
